odd_indexed_indices_reorder symmetric

crypto_examples/index.dfy
@@ -142,17 +142,6 @@ module rindex {
             && idxs[i].bins[..offset] == idxs[j].bins[..offset])
     }
 
-    // lemma ntt_indicies_lower_bits_equal(idxs: seq<index_t>, len: pow2_t, k: nat)
-    //     requires k < pow2(L - len.exp)
-    //     requires len.full <= N
-    //     requires ntt_indicies_wf(idxs, len)
-    //     // requires idxs[i].bins[..offset] == 
-    // {
-    //     var offset := L - len.exp;
-    //     forall i, j :: 0 <= i < len.full && 0 <= j < len.full
-    //         ensures 
-    // }
-
     // base case happens at level 1, chuck size is the whole array
     lemma ntt_indicies_inv_base_case(idxs: seq<index_t>, len: pow2_t, k: nat)
         requires len == pow2(L) 
@@ -369,55 +358,169 @@ module rindex {
         }
     }
 
-//     function method odd_indexed_indices(idxs: seq<index_t>, len: pow2_t): (idx': seq<index_t>)
-//         requires |idxs| == len.full >= 2;
-//         ensures |idx'| == len.full / 2;
-//     {
-//         pow2_basics(len);
-//         seq(len.full/2, n requires 0 <= n < len.full/2 => idxs[n * 2 + 1])
-//     }
+    function method odd_indexed_indices(idxs: seq<index_t>, len: pow2_t): (idx': seq<index_t>)
+        requires |idxs| == len.full >= 2;
+        ensures |idx'| == len.full / 2;
+    {
+        pow2_basics(len);
+        seq(len.full/2, n requires 0 <= n < len.full/2 => idxs[n * 2 + 1])
+    }
 
-//    lemma odd_indexed_indices_reorder(idxs: seq<index_t>, len: pow2_t, idxs': seq<index_t>)
-//         requires len.full >= 2;
-//         requires ntt_indicies_inv(idxs, len); 
-//         requires odd_indexed_indices(idxs, len) == idxs';
-//         ensures ntt_indicies_inv(idxs', pow2_half(len));
-//     {
-//         var len' := pow2_half(len);
-//         assert ntt_indicies_wf(idxs', len');
+    lemma odd_indexed_indices_reorder(idxs: seq<index_t>, len: pow2_t, idxs': seq<index_t>, k: nat)
+        requires len.full >= 2;
+        requires ntt_indicies_inv(idxs, len, k); 
+        requires k < pow2_div(pow2(L), len).full
+        requires odd_indexed_indices(idxs, len) == idxs';
+        ensures ntt_indicies_inv(idxs', pow2_half(len), k * 2 + 1);
+    {
+        var len' := pow2_half(len);
+        assert ntt_indicies_wf(idxs', len');
 
-//         forall i: nat | i < len'.full
-//             ensures ToNatRight(idxs'[i].bins[(L - len'.exp)..]) == i
-//         {
-//             var bins := idxs[i * 2 + 1].bins;
-//             assert bins == idxs'[i].bins;
+        var offset := L - len.exp;
+        var offset' := offset + 1;
 
-//             var offset := L - len.exp;
-//             var prev := bins[offset..];
-//             var curr := bins[offset'..];
+        forall i: nat | i < len'.full
+            ensures ToNatRight(idxs'[i].bins[offset'..]) == i
+            ensures idxs'[i].bins[offset] == 1
+        {
+            var bins := idxs[i * 2+1].bins;
+            assert bins == idxs'[i].bins;
 
-//             calc == {
-//                 2 * i + 1;
-//                 ToNatRight(prev);
-//                 {
-//                     assert [bins[offset]] + curr == prev;
-//                     assert DropFirst(prev) == curr;
-//                     reveal ToNatRight();
-//                 }
-//                 ToNatRight(curr) * 2 + bins[offset];
-//                 {
-//                     LemmaSeqLswModEquivalence(prev);
-//                     assert ToNatRight(prev) == 2 * i + 1;
-//                     assert bins[offset] == 1;
-//                 }
-//                 ToNatRight(curr) * 2 + 1;
-//             }
+            var prev := bins[offset..];
+            var curr := bins[offset'..];
 
-//             calc == {
-//                 i;
-//                 ToNatRight(curr);
-//                 ToNatRight(idxs'[i].bins[(L - len'.exp)..]);
-//             }
-//         }
-//     }
+            calc == {
+                2 * i + 1;
+                ToNatRight(prev);
+                {
+                    assert [bins[offset]] + curr == prev;
+                    assert DropFirst(prev) == curr;
+                    reveal ToNatRight();
+                }
+                ToNatRight(curr) * 2 + bins[offset];
+            }
+
+            assert bins[offset] == 1 by {
+                LemmaSeqLswModEquivalence(prev);
+                assert ToNatRight(prev) == 2 * i + 1;
+            }
+
+            assert 2 * i == ToNatRight(curr) * 2;
+
+            calc == {
+                i;
+                ToNatRight(curr);
+                ToNatRight(idxs'[i].bins[offset'..]);
+            }
+        }
+
+        forall i: nat, j: nat | i < len'.full && j < len'.full
+            ensures idxs'[i].bins[..offset'] == idxs'[j].bins[..offset']
+        {
+            var i_bins := idxs[i * 2+1].bins;
+            assert i_bins == idxs'[i].bins;
+
+            var j_bins := idxs[j * 2+1].bins;
+            assert j_bins == idxs'[j].bins;
+
+            assert i_bins[..offset] == j_bins[..offset];
+
+            calc == {
+                i_bins[..offset'];
+                i_bins[..offset] + [i_bins[offset]];
+                i_bins[..offset] + [1];
+                j_bins[..offset] + [j_bins[offset]];
+                j_bins[..offset'];
+            }
+        }
+
+        var k' := k * 2 + 1;
+
+        calc {
+            k';
+            k * 2 + 1;
+        <   
+            pow2(L - len.exp).full * 2 + 1;
+            { pow2_basics(pow2(1)); }
+            pow2(L - len.exp).full * pow2(1).full + 1;
+            { var _ := pow2_mul(pow2(L - len.exp), pow2(1)); }
+            pow2(L - len.exp + 1).full + 1;
+            pow2(L - len'.exp).full + 1;
+            { var _ := pow2_div(pow2(L), pow2(len.exp)); }
+            pow2_div(pow2(L), len').full + 1;
+        }
+
+        assert k' < pow2_div(pow2(L), len').full by {
+            pow2_basics(pow2_div(pow2(L), len'));
+            assert k' != pow2_div(pow2(L), len').full;
+        }
+
+        forall i: nat | i < len'.full
+            ensures idxs'[i].bins[..offset'] ==
+                Reverse(orignal_index(k', i, len').bins[len'.exp..])
+        {
+            pow2_basics(len);
+
+            var orignal := orignal_index(k', i, len');
+
+            calc == {
+                orignal.v;
+                k' * len'.full + i;
+                (2 * k + 1) * (len.full / 2) + i;
+                {
+                    LemmaMulIsDistributiveAuto();
+                }
+                2 * k * (len.full / 2) + len.full / 2 + i;
+                {
+                    LemmaMulIsAssociativeAuto();
+                }
+                k * (2 * (len.full / 2)) + len.full / 2 + i;
+                k * len.full + len.full / 2 + i;
+                k * len.full + len'.full + i;
+            }
+    
+            assert orignal_index(k, len'.full + i, len) == orignal;
+
+            // calc == {
+            //     idxs'[i].bins[..offset];
+            //     idxs[i].bins[..offset];
+            //     Reverse(orignal.bins[len.exp..]);
+            // }
+    
+            var obins := orignal.bins;
+
+            calc == {
+                obins[len.exp-1];
+                {
+                    BitSelModEquivalence(obins, len.exp-1);
+                }
+                (ToNatRight(obins) / Pow(2, len.exp-1)) % 2;
+                {
+                    assert Pow(2, len.exp-1) == Pow(2, len'.exp);
+                    reveal Pow2();
+                    assert Pow(2, len'.exp) == len'.full;
+                }
+                (orignal.v / len'.full) % 2;
+                ((k' * len'.full + i) / len'.full) % 2;
+                {
+                    LemmaFundamentalDivModConverse(orignal.v, len'.full, k', i);
+                    assert (k' * len'.full + i) / len'.full == k';
+                }
+                k' % 2;
+                1;
+            }
+
+            calc == {
+                Reverse(obins[len'.exp..]);
+                Reverse(obins[len.exp-1..]);
+                {
+                    SubSeqReverseProperty(obins, len.exp);
+                }
+                Reverse(obins[len.exp..]) + [obins[len.exp-1]];
+                idxs'[i].bins[..offset] + [obins[len.exp-1]];
+                idxs'[i].bins[..offset] + [1];
+                idxs'[i].bins[..offset'];
+            }
+        }
+    }
 }
